Un-layer the TreeSync proofs ; give better module names

fstar/MLS.TreeSync.Refined.Operations.fst
@@ -1,4 +1,4 @@
-module MLS.TreeSync.Level2
+module MLS.TreeSync.Refined.Operations
 
 open Comparse
 open MLS.Crypto
@@ -6,10 +6,10 @@ open MLS.NetworkTypes
 open MLS.TreeSync.NetworkTypes
 open MLS.Tree
 open MLS.TreeCommon
-open MLS.TreeSync.Level0
-open MLS.TreeSync.Level1
-open MLS.TreeSync.Level1.Proofs
-open MLS.TreeSync.Level2.Types
+open MLS.TreeSync.Operations
+open MLS.TreeSync.Invariants.UnmergedLeaves.Proofs
+open MLS.TreeSync.Invariants.ParentHash.Proofs
+open MLS.TreeSync.Refined.Types
 
 val tree_add_pre: #bytes:Type0 -> {|crypto_bytes bytes|} -> #tkt:treekem_types bytes -> #l:nat -> #i:tree_index l -> treesync bytes tkt l i -> li:leaf_index l i -> bool
 let tree_add_pre #bytes #cb #tkt #l #i t li = tree_add_pre t li
@@ -18,16 +18,19 @@ val tree_add: #bytes:Type0 -> {|crypto_bytes bytes|} -> #tkt:treekem_types bytes
   (requires tree_add_pre t li)
   (ensures fun _ -> True)
 let tree_add #bytes #cb #tkt #l #i t li ln =
+  unmerged_leaves_ok_tree_add t li ln;
   parent_hash_invariant_tree_add t li ln;
   tree_add t li ln
 
 val tree_update: #bytes:Type0 -> {|crypto_bytes bytes|} -> #tkt:treekem_types bytes -> #l:nat -> #i:tree_index l -> t:treesync bytes tkt l i -> li:leaf_index l i -> leaf_node_nt bytes tkt -> treesync bytes tkt l i
 let tree_update #bytes #cb #tkt #l #i t li ln =
+  unmerged_leaves_ok_tree_update t li ln;
   parent_hash_invariant_tree_update t li ln;
   tree_update t li ln
 
 val tree_remove: #bytes:Type0 -> {|crypto_bytes bytes|} -> #tkt:treekem_types bytes -> #l:nat -> #i:tree_index l -> t:treesync bytes tkt l i -> li:leaf_index l i -> treesync bytes tkt l i
 let tree_remove #bytes #cb #tkt #l #i t li =
+  unmerged_leaves_ok_tree_remove t li;
   parent_hash_invariant_tree_remove t li;
   tree_remove t li
 
@@ -39,20 +42,24 @@ val apply_external_path: #bytes:Type0 -> {|crypto_bytes bytes|} -> #tkt:treekem_
   (requires apply_external_path_pre t p /\ external_path_is_parent_hash_valid t p /\ external_path_is_filter_valid t p)
   (ensures fun _ -> True)
 let apply_external_path #bytes #cb #tkt #l #li t p =
+  unmerged_leaves_ok_apply_external_path t p;
   parent_hash_invariant_apply_external_path t p;
   apply_external_path t p
 
 val mk_blank_tree: #bytes:Type0 -> {|crypto_bytes bytes|} -> #tkt:treekem_types bytes -> l:nat -> i:tree_index l -> treesync bytes tkt l i
 let mk_blank_tree #bytes #cb #tkt l i =
+  unmerged_leaves_ok_mk_blank_tree #bytes #cb.base #tkt l i;
   parent_hash_invariant_mk_blank_tree #bytes #cb #tkt l i;
   mk_blank_tree l i
 
 val tree_extend: #bytes:Type0 -> {|crypto_bytes bytes|} -> #tkt:treekem_types bytes -> #l:nat -> t:treesync bytes tkt l 0 -> treesync bytes tkt (l+1) 0
 let tree_extend #bytes #cb #tkt #l t =
+  unmerged_leaves_ok_tree_extend t;
   parent_hash_invariant_tree_extend t;
   tree_extend t
 
 val tree_truncate: #bytes:Type0 -> {|crypto_bytes bytes|} -> #tkt:treekem_types bytes -> #l:pos -> t:treesync bytes tkt l 0{is_tree_empty (TNode?.right t)} -> treesync bytes tkt (l-1) 0
 let tree_truncate #bytes #cb #tkt #l t =
+  unmerged_leaves_ok_tree_truncate t;
   parent_hash_invariant_tree_truncate t;
   tree_truncate t
