fstar/MLS.TreeSync.Refined.Types.fst
@@ -1,0 +1,13 @@
+module MLS.TreeSync.Refined.Types
+
+open MLS.Crypto
+open MLS.Tree
+open MLS.TreeSync.NetworkTypes
+open MLS.TreeSync.Types
+open MLS.TreeSync.Invariants.UnmergedLeaves
+open MLS.TreeSync.Invariants.ParentHash
+
+let treesync (bytes:Type0) {|crypto_bytes bytes|} (tkt:treekem_types bytes) (l:nat) (i:tree_index l) =
+  t:treesync bytes tkt l i{unmerged_leaves_ok t /\ parent_hash_invariant t}
+
+let external_pathsync = external_pathsync
